src/program_proof/pav/rpc.v
@@ -223,8 +223,8 @@ Module servPutReply.
 Record t :=
   mk {
     putEpoch: w64;
-    prev2Link: list w8;
-    prevDig: list w8;
+    prevLink: list w8;
+    dig: list w8;
     linkSig: list w8;
     putSig: list w8;
     error: bool;
@@ -234,25 +234,18 @@ Section local_defs.
 Context `{!heapGS Σ, !mono_listG (list w8) Σ, !mono_listG gname Σ, !ghost_mapG Σ (list w8) (list w8)}.
 
 Definition own ptr obj : iProp Σ :=
-  ∃ sl_prev2Link sl_prevDig sl_linkSig sl_putSig d0 d1 d2 d3,
+  ∃ sl_prevLink sl_dig sl_linkSig sl_putSig d0 d1 d2 d3,
   "Herror" ∷ ptr ↦[servPutReply :: "error"] #obj.(error) ∗
   if negb obj.(error) then
     "HputEpoch" ∷ ptr ↦[servPutReply :: "putEpoch"] #obj.(putEpoch) ∗
-    "Hprev2Link" ∷ ptr ↦[servPutReply :: "prev2Link"] (slice_val sl_prev2Link) ∗
-    "Hsl_prev2Link" ∷ own_slice_small sl_prev2Link byteT d0 obj.(prev2Link) ∗
-    "HprevDig" ∷ ptr ↦[servPutReply :: "prevDig"] (slice_val sl_prevDig) ∗
-    "Hsl_prevDig" ∷ own_slice_small sl_prevDig byteT d1 obj.(prevDig) ∗
+    "HprevLink" ∷ ptr ↦[servPutReply :: "prevLink"] (slice_val sl_prevLink) ∗
+    "Hsl_prevLink" ∷ own_slice_small sl_prevLink byteT d0 obj.(prevLink) ∗
+    "Hdig" ∷ ptr ↦[servPutReply :: "dig"] (slice_val sl_dig) ∗
+    "Hsl_dig" ∷ own_slice_small sl_dig byteT d1 obj.(dig) ∗
     "HlinkSig" ∷ ptr ↦[servPutReply :: "linkSig"] (slice_val sl_linkSig) ∗
     "Hsl_linkSig" ∷ own_slice_small sl_linkSig byteT d2 obj.(linkSig) ∗
     "HputSig" ∷ ptr ↦[servPutReply :: "putSig"] (slice_val sl_putSig) ∗
     "Hsl_putSig" ∷ own_slice_small sl_putSig byteT d3 obj.(putSig)
-    (* Valid sigpreds, proving that the server completed the op. *)
-    (*
-    "#HprevLink" ∷ is_hash (chainSepSome.encodesF (chainSepSome.mk (word.sub obj.(putEpoch) (W64 1)) obj.(prev2Link) obj.(prevDig))) prevLink ∗
-    "Hlink_sigpred" ∷ serv_sigpred_link γmonoLinks (servSepLink.mk prevLink) ∗
-    "Hput_sigpred" ∷ serv_sigpred_put γmonoTrees (servSepPut.mk obj.(putEpoch) id val)
-    *)
   else True.
-
 End local_defs.
 End servPutReply.
