src/program_proof/pav/server.v
@@ -58,9 +58,9 @@ Definition own ptr obj : iProp Σ :=
     epochInfo.own ptr_epoch epoch).
 
 Definition valid pk γtrees obj : iProp Σ :=
-  "#Hsep_valid" ∷ ([∗ list] k ↦ γtree; info ∈ γtrees; obj.(epochs),
+  "#Hvalid_sep_chain" ∷ ([∗ list] k ↦ γtree; info ∈ γtrees; obj.(epochs),
     epochInfo.valid pk k γtree info) ∗
-  "#Hbinds" ∷ binds (epochInfo.dig <$> obj.(epochs)) (epochInfo.link <$> obj.(epochs)).
+  "#Hbinds_chain" ∷ binds (epochInfo.dig <$> obj.(epochs)) (epochInfo.link <$> obj.(epochs)).
 End defs.
 End epochChain.
 
@@ -69,36 +69,59 @@ Record t :=
   mk {
     mu: loc;
     γ: gname;
+    sl_sk: Slice.t;
+    pk: list w8;
   }.
 
-Section local_defs.
+Section defs.
 Context `{!heapGS Σ, !pavG Σ}.
 
 Definition own ptr obj : iProp Σ :=
-  ∃ ptr_updates (updates : gmap (list w8) (list w8)) map_sl_updates ptr_chain γtrees γupdates sl_sk pk chain,
+  ∃ ptr_updates (updates : gmap (list w8) (list w8)) sl_updates ptr_chain γtrees γupdates chain,
   (* ghost state, the other half owned by global_inv. *)
   "HmonoTrees" ∷ mono_list_auth_own obj.(γ) (1/2) (γtrees ++ [γupdates]) ∗
   "Hupdates_view" ∷ ghost_map_auth γupdates (1/2) updates ∗
 
-  "Hsk" ∷ ptr ↦[server :: "sk"] (slice_val sl_sk) ∗
-  "Hown_sk" ∷ own_sk sl_sk pk (serv_sigpred obj.(γ)) ∗
+  "Hown_sk" ∷ own_sk obj.(sl_sk) obj.(pk) (serv_sigpred obj.(γ)) ∗
 
   "Hown_chain" ∷ epochChain.own ptr_chain chain ∗
-  "#Hvalid_chain" ∷ epochChain.valid pk γtrees chain ∗
+  "%Hlen_nz_chain" ∷ ⌜ length chain.(epochChain.epochs) > 0 ⌝ ∗
+  "#Hvalid_chain" ∷ epochChain.valid obj.(pk) γtrees chain ∗
   "Hptr_chain" ∷ ptr ↦[server :: "chain"] #ptr_chain ∗
 
-  (* exists map of slices that own the respective vals. *)
-  "Hmap_sl_updates" ∷ ([∗ map] sl_bytes; bytes ∈ map_sl_updates; (kmap bytes_to_string updates),
-    own_slice_small sl_bytes byteT (DfracOwn 1) bytes) ∗
-  "Hown_updates" ∷ own_map ptr_updates (DfracOwn 1) map_sl_updates ∗
+  (* exists (idS, sl_v) map that owns the respective (id, v) map. *)
+  "#Hsl_updates" ∷ ([∗ map] sl_v; v ∈ sl_updates; (kmap bytes_to_string updates),
+    own_slice_small sl_v byteT DfracDiscarded v) ∗
+  "Hown_updates" ∷ own_map ptr_updates (DfracOwn 1) sl_updates ∗
   "Hupdates" ∷ ptr ↦[server :: "updates"] #ptr_updates.
 
 Definition valid ptr obj : iProp Σ :=
-  "#Hmu" ∷ ptr ↦[server :: "mu"]□ #obj.(mu) ∗
+  "#Hptr_mu" ∷ ptr ↦[server :: "mu"]□ #obj.(mu) ∗
   "#HmuR" ∷ is_lock nroot #obj.(mu) (own ptr obj) ∗
-  "#Hinv" ∷ inv nroot (global_inv obj.(γ)).
-End local_defs.
+  "#Hinv" ∷ inv nroot (global_inv obj.(γ)) ∗
+  "#ptr_Hsk" ∷ ptr ↦[server :: "sk"]□ (slice_val obj.(sl_sk)).
+End defs.
 End server.
+
+Section misc.
+Context `{!heapGS Σ, !pavG Σ}.
+Definition servPutReply_valid pk id val (obj : servPutReply.t) : iProp Σ :=
+  (if negb obj.(servPutReply.error) then
+    ∃ link,
+    "#Hlink" ∷ is_hash
+      (chainSepSome.encodesF (chainSepSome.mk
+        (word.sub obj.(servPutReply.putEpoch) (W64 1))
+        obj.(servPutReply.prevLink)
+        obj.(servPutReply.dig)))
+      link ∗
+    "#Hvalid_linkSig" ∷ is_sig pk
+      (servSepLink.encodesF (servSepLink.mk link))
+      obj.(servPutReply.linkSig) ∗
+    "#Hvalid_putSig" ∷ is_sig pk
+      (servSepPut.encodesF (servSepPut.mk obj.(servPutReply.putEpoch) id val))
+      obj.(servPutReply.putSig)
+  else True)%I.
+End misc.
 
 Section proofs.
 Context `{!heapGS Σ, !pavG Σ}.
@@ -142,7 +165,8 @@ Lemma wp_server_put ptr_serv obj_serv sl_id sl_val (id val : list w8) d0 d1 :
   server__put #ptr_serv (slice_val sl_id) (slice_val sl_val)
   {{{
     ptr_reply reply, RET #ptr_reply;
-    "Hreply" ∷ servPutReply.own ptr_reply reply obj_serv.(server.γmonoLinks) obj_serv.(server.γmonoTrees) id val
+    "Hown_reply" ∷ servPutReply.own ptr_reply reply ∗
+    "#Hvalid_reply" ∷ servPutReply_valid obj_serv.(server.pk) id val reply
   }}}.
 Proof.
   rewrite /server__put.
@@ -151,20 +175,24 @@ Proof.
   wp_loadField.
   wp_apply (acquire_spec with "[$HmuR]"); iIntros "[Hlocked Hown_serv]"; iNamed "Hown_serv".
 
+  (* error val. *)
   wp_apply wp_allocStruct; [val_ty|];
     iIntros (ptr_errReply) "Hptr_errReply".
-  iDestruct (struct_fields_split with "Hptr_errReply") as "H"; iNamed "H".
+  iDestruct (struct_fields_split with "Hptr_errReply") as "H";
+    iNamed "H"; iClear "putEpoch prevLink dig linkSig putSig".
   wp_storeField.
-  iAssert (servPutReply.own ptr_errReply (servPutReply.mk 0 [] [] [] [] _) obj_serv.(server.γmonoLinks) obj_serv.(server.γmonoTrees) id val) with "[$error //]" as "HerrReply".
+  set (errReply := servPutReply.mk 0 [] [] [] [] true).
+  iAssert (servPutReply.own ptr_errReply errReply) with "[$error //]" as "Hown_errReply".
+  iAssert (servPutReply_valid obj_serv.(server.pk) id val errReply) with "[//]" as "#Hvalid_errReply".
 
   (* check id len. *)
   wp_apply wp_slice_len.
   wp_if_destruct.
   {
     wp_loadField.
-    (* TODO: debug why this iFrame takes so long. *)
-    wp_apply (release_spec with "[-HΦ HerrReply]"); [iFrame "#∗#"|].
-    wp_pures; by iApply "HΦ".
+    wp_apply (release_spec with "[-HΦ Hown_errReply]").
+    1: iFrame "HmuR Hlocked"; iFrame "∗#%".
+    wp_pures; iApply "HΦ"; by iFrame.
   }
 
   (* check if id was already updated. if not, update. *)
@@ -175,146 +203,111 @@ Proof.
   destruct ok.
   {
     wp_loadField.
-    wp_apply (release_spec with "[-HΦ HerrReply]"); [iFrame "#∗#"|].
-    wp_pures; by iApply "HΦ".
+    wp_apply (release_spec with "[-HΦ Hown_errReply]").
+    1: iFrame "HmuR Hlocked"; iFrame "∗#%".
+    wp_pures; iApply "HΦ"; by iFrame.
   }
   wp_loadField.
   wp_apply (wp_MapInsert_to_val with "[$Hown_updates]"); iIntros "Hown_updates".
 
   (* prepare put promise. *)
   wp_loadField.
+  iNamed "Hown_chain".
+  wp_loadField.
   wp_apply wp_slice_len.
-  wp_pures.
   wp_apply wp_allocStruct; [val_ty|];
     iIntros (ptr_putPre_obj) "Hptr_putPre_obj".
-  wp_apply (servSepPut.wp_encode with "[Hptr_putPre_obj Hid Hval]").
+  iMod (own_slice_small_persist with "Hval") as "#Hval".
+  wp_apply (servSepPut.wp_encode with "[Hptr_putPre_obj Hid]").
   {
     iDestruct (struct_fields_split with "Hptr_putPre_obj") as "H"; iNamed "H".
     instantiate (1:=servSepPut.mk _ _ _).
     rewrite /servSepPut.own /=.
-    iExists sl_id, sl_val; iFrame.
+    iExists sl_id, sl_val; iFrame "∗#".
   }
   iIntros (sl_putPre putPre) "H"; iNamed "H";
     iRename "Hobj" into "Hptr_putPre";
     iRename "Hsl_enc" into "Hsl_putPre";
     move: Henc => Henc_putPre.
-  replace (word.add (word.sub sl_ptr_trees.(Slice.sz) (W64 1)) (W64 1)) with (sl_ptr_trees.(Slice.sz)) in Henc_putPre by ring.
+  replace (word.add (word.sub sl_epochs.(Slice.sz) (W64 1)) (W64 1)) with (sl_epochs.(Slice.sz)) in * by ring.
+  wp_loadField.
+  (* load chain lengths. *)
+  iNamed "Hvalid_chain".
+  iDestruct (big_sepL2_length with "Hvalid_sep_chain") as %Hlen_gammas_chain.
+  iDestruct (own_slice_small_sz with "Hsl_epochs") as %Hlen_sl_epochs.
+  iDestruct (big_sepL2_length with "Hsep_epochs") as %Hlen_ptr_epochs.
 
   (* get resources for put sigpred. *)
   (* get γtree mono_list_idx_own. *)
-  iDestruct (own_slice_small_sz with "Hsl_ptr_trees") as %Hlen0.
-  iDestruct (big_sepL2_length with "Hown_trees") as %Hlen1.
-  iDestruct (big_sepL2_length with "Htree_views") as %Hlen2.
-  rewrite app_length/= in Hlen2.
-  assert (uint.nat sl_ptr_trees.(Slice.sz) < length γtrees) as Hinb by lia.
-  apply lookup_lt_is_Some in Hinb as [γtree Hlook0].
-  iDestruct (mono_list_idx_own_get with "[HmonoTrees]") as "#Hidx_γtree".
+  iDestruct (mono_list_idx_own_get (uint.nat sl_epochs.(Slice.sz)) γupdates with "[HmonoTrees]") as "#Hidx_γupdates".
   2: iApply (mono_list_lb_own_get with "HmonoTrees").
-  1: done.
-  (* open invariant to get even more info. *)
+  1: { apply lookup_snoc_Some; eauto with lia. }
+  (* open global_inv. *)
   wp_apply ncfupd_wp.
   iRename "HmonoTrees" into "HmonoTrees0".
-  iRename "Htree_views" into "Htree_views0".
-  iInv "Hinv" as "> H" "Hclose".
-  iEval (rewrite /global_inv) in "H".
-  (* TODO: very weird...
-     if we do `iNamed "H".` here with a conflicting hyp name,
-     instead of error'ing out, our goal becomes False.
-     this seems like bad behavior from iris_named_props. *)
-  iRename "Hdigs" into "Hdigs0".
-  iNamed "H".
+  iInv "Hinv" as "> H" "Hclose"; iNamed "H".
+  (* get ghost_map_auth updates in full, so we can update and make put witness. *)
   iDestruct (mono_list_auth_own_agree with "HmonoTrees HmonoTrees0") as %[_ ->].
-  iDestruct (sep_auth_agree with "Htree_views Htree_views0") as %?; list_simplifier.
-  (* get ghost map witness. *)
-  assert ((trees ++ [updates]) !! uint.nat sl_ptr_trees.(Slice.sz) = Some updates) as Hlook1.
-  { apply lookup_snoc_Some; eauto with lia. }
-  iDestruct (big_sepL2_insert_acc with "Htree_views0") as "[Hmap_auth0 Hsep_close0]"; [done..|].
-  iDestruct (big_sepL2_insert_acc with "Htree_views") as "[Hmap_auth1 Hsep_close1]"; [done..|].
-  iCombine "Hmap_auth0 Hmap_auth1" as "Hmap_auth".
+  iDestruct (big_sepL2_snoc with "Htree_views") as "[Htree_views Hupdates_view0]".
+  iDestruct (ghost_map_auth_agree with "Hupdates_view0 Hupdates_view") as %->.
+  iCombine "Hupdates_view Hupdates_view0" as "Hupdates_view".
   apply map_get_false in Hmap_get as [Hmap_get _].
-  iDestruct (big_sepM2_lookup_l_none with "Hmap_sl_updates") as "%Hmap_get1"; [done|].
+  iDestruct (big_sepM2_lookup_l_none with "Hsl_updates") as "%Hmap_get1"; [done|].
   rewrite lookup_kmap in Hmap_get1.
-  iMod (ghost_map_insert_persist _ val with "Hmap_auth") as "[[Hmap_auth0 Hmap_auth1] #Hwitness]"; [done|].
-  (* make resources look pretty before closing invariant. *)
-  iDestruct ("Hsep_close0" with "Hmap_auth0") as "Htree_views0".
-  iDestruct ("Hsep_close1" with "Hmap_auth1") as "Htree_views1".
-  pose proof (list_insert_id _ _ _ Hlook0) as H;
-    iEval (rewrite H) in "Htree_views0 Htree_views1";
-    clear H.
-  assert (uint.nat sl_ptr_trees.(Slice.sz) = length trees + 0) as H by lia;
-    iEval (rewrite H insert_app_r) in "Htree_views0 Htree_views1";
-    list_simplifier; clear H.
-  iMod ("Hclose" with "[$Hlinks $HmonoTrees $Htree_views1]") as "_"; [iFrame "%#"|].
-  iClear "Hbinds Hdigs".
+  iMod (ghost_map_insert_persist _ val with "Hupdates_view") as "[[Hupdates_view0 Hupdates_view1] #Hwitness]"; [done|].
+  iDestruct (big_sepL2_snoc with "[$Htree_views $Hupdates_view0]") as "Htree_views".
+  iMod ("Hclose" with "[$HmonoTrees0 $Htree_views]") as "_"; [iFrame "#"|].
+  iClear "Hdigs Hdigs_links".
 
   (* sign put promise. *)
   iModIntro.
-  wp_loadField.
   wp_apply (wp_Sign with "[$Hown_sk $Hsl_putPre]").
-  {
-    iRight.
-    (* TODO: with iFrame "%", it's unfolding mono_list_idx_own,
-       framing the lookup, and left with a mono_list_lb_own, which we don't have.
-       maybe mono_list_idx_own should be more opaque? *)
-    iFrame (Henc_putPre).
-    iFrame "#".
-  }
-  iIntros (sl_putSig putSig) "H";
-    iRename "Hsk" into "Hptr_sk";
-    iNamed "H";
+  1: iFrame "Hinv"; iRight; iFrame "%#".
+  iIntros (sl_putSig putSig) "H"; iNamed "H";
     iRename "Hmsg" into "Hsl_putPre";
-    iRename "Hsig" into "HputSig".
+    iRename "Hsig" into "Hvalid_putSig";
+    iRename "Hsl_sig" into "Hsl_putSig".
 
-  (* get all the other data to be returned. *)
+  (* extract resources from chain and return. *)
   wp_loadField.
-  wp_apply (hashChain.wp_getLink with "Hown_chain"); [admit|].
-  iIntros (sl_prev2Link prev2Link) "H";
-    iRename "Hchain" into "Hptr_chain";
-    iNamed "H".
-  remember (word.sub sl_ptr_trees.(Slice.sz) (W64 1)) as currEpoch.
-  remember (word.sub currEpoch (W64 1)) as prevEpoch.
-  assert (links !! uint.nat prevEpoch = Some prev2Link) as Hlook2 by admit.
-  (* TODO: prove by showing in bounds in (drop 1 links) and extracting
-     from mono_list_auth_own. *)
-  iAssert ((⌜ uint.nat currEpoch > 0 ⌝ -∗ mono_list_idx_own obj_serv.(server.γmonoLinks) (uint.nat prevEpoch) prev2Link)%I) as "Hmono_prev2Link"; [admit|].
-
   wp_loadField.
-  assert (∃ ptr_tree, ptr_trees !! uint.nat currEpoch = Some ptr_tree) as [ptr_tree Hlook3] by admit.
-  wp_apply (wp_SliceGet with "[$Hsl_ptr_trees //]"); iIntros "Hsl_ptr_trees".
-  iDestruct (big_sepL2_lookup_1_some with "Hown_trees") as %[tree Htree]; [done|].
-  iDestruct (big_sepL2_lookup_acc with "Hown_trees") as "[Hown_tree Hown_trees_close]"; [done..|].
-  wp_apply (wp_Tree_Digest with "Hown_tree");
-    iIntros (sl_prevDig prevDig) "H"; iNamed "H".
-  assert (digs !! uint.nat currEpoch = Some prevDig) as Hlook4 by admit.
-  assert (∃ prevLink, links !! uint.nat currEpoch = Some prevLink) as [prevLink Hlook5] by admit.
-  iAssert (is_hash (chainSepSome.encodesF (chainSepSome.mk currEpoch prev2Link prevDig)) prevLink) as "Hbind_prevLink"; [admit|].
-  iAssert (mono_list_idx_own obj_serv.(server.γmonoLinks) (uint.nat currEpoch) prevLink) as "Hmono_prevLink"; [admit|].
-
+  pose proof (lookup_lt_is_Some ptr_epochs (uint.nat (word.sub sl_epochs.(Slice.sz) (W64 1)))) as [_ H];
+    unshelve (epose proof (H _) as [ptr_epoch Hidx_ptr_epoch]);
+    [word|]; clear H.
+  wp_apply (wp_SliceGet with "[$Hsl_epochs //]"); iIntros "Hsl_epochs".
+  iDestruct (big_sepL2_lookup_1_some with "Hsep_epochs") as %[chain_epoch Hidx_chain]; [done|].
+  iDestruct (big_sepL2_lookup_acc with "Hsep_epochs") as "[Hown_epoch Hsep_epochs]"; [done..|].
+  iNamed "Hown_epoch".
+  iMod (own_slice_small_persist with "Hsl_prevLink") as "#Hsl_prevLink".
+  iMod (own_slice_small_persist with "Hsl_dig") as "#Hsl_dig".
+  iMod (own_slice_small_persist with "Hsl_linkSig") as "#Hsl_linkSig".
   wp_loadField.
-  iDestruct "Hown_linkSigs" as (linkSigs_dim0) "[HlinkSigs_dim0 Hown_linkSigs]".
-  assert (∃ sl_linkSig, linkSigs_dim0 !! uint.nat currEpoch = Some sl_linkSig) as [sl_linkSig Hlook6] by admit.
-  wp_apply (wp_SliceGet with "[$HlinkSigs_dim0]"); [done|];
-    iIntros "HlinkSigs_dim0".
-
-  (* return. *)
   wp_loadField.
-  iDestruct ("Hown_trees_close" with "Htree") as "Hown_trees".
-  iAssert (own_Slice2D sl_linkSigs (DfracOwn 1) linkSigs) with "[$Hown_linkSigs $HlinkSigs_dim0]" as "Hown_linkSigs".
-  wp_apply (release_spec with "[Hlocked Hptr_sk HlinkSigs Hptr_chain HmonoLinks Hmap_sl_updates Hupdates Htrees HmonoTrees0 Hown_updates Htree_views0 Hsk Hchain Hsl_ptr_trees Hown_trees Hown_linkSigs]"); [admit|].
+  wp_loadField.
+  iDestruct ("Hsep_epochs" with "[$Htr $Hsl_link $Hptr_tr $Hptr_prevLink
+    $Hptr_dig $Hptr_link $Hptr_linkSig]") as "Hsep_epochs"; [iFrame "#"|].
+  iRename "Hsl_updates" into "H";
+    iDestruct (big_sepM2_insert_2 _ _ _ (bytes_to_string id) with "[] H")
+    as "Hsl_updates"; [iFrame "Hval"|]; iClear "H".
+  iEval (rewrite -kmap_insert) in "Hsl_updates".
+  wp_loadField.
+  wp_apply (release_spec with "[-HΦ Hptr_putPre Hsl_putPre Hsl_putSig]").
+  1: iFrame "Hlocked HmuR"; iFrame "∗#%".
   wp_apply wp_allocStruct; [val_ty|];
     iIntros (ptr_putReply) "Hptr_putReply".
-  iClear "putEpoch prev2Link prevDig linkSig putSig HerrReply".
   iDestruct (struct_fields_split with "Hptr_putReply") as "H"; iNamed "H".
+  replace (word.add (word.sub sl_epochs.(Slice.sz) (W64 1)) (W64 1)) with (sl_epochs.(Slice.sz)) in * by ring.
   iApply "HΦ".
+  iFrame.
   instantiate (1:=servPutReply.mk _ _ _ _ _ _).
   rewrite /servPutReply.own /=.
-  iExists prevLink, sl_prev2Link, sl_prevDig, sl_linkSig, sl_putSig.
   iFrame "∗#".
-  (*
-     first get mono_idx for prevLink.
-     then just need to unify bindings and exhibit mono_idx.
-   *)
-Admitted.
+  iDestruct (big_sepL2_lookup_2_some with "Hvalid_sep_chain") as %[γtree Hidx_γtree]; [done|].
+  iDestruct (big_sepL2_lookup with "Hvalid_sep_chain") as "H"; [done..|]; iNamed "H".
+  iEval (rewrite w64_to_nat_id) in "Hbind".
+  rewrite /servSepPut.encodes in Henc_putPre; subst.
+  iFrame "#".
+Qed.
 
 Lemma wp_server_updateEpoch ptr_serv obj_serv :
   {{{
